tutorial/BasicLoops.v
@@ -27,6 +27,9 @@ Require Export Picinae_simplifier_v1_1.
 Require Import Picinae_pilbox32.
 Require Import NArith.
 Require Import Structures.Equalities.
+Require Import Lia ZifyN.
+Require Import Utf8.
+Import PIL32Notations.
 Open Scope N.
 Ltac fail_seek ::= idtac.
 
@@ -50,11 +53,19 @@ Module Addloop.
 Module Addloop1.
 Definition addloop (s:store) (a:addr) : option (N * stmt) :=
   match a with
+    (* nop *)
   | 100 => Some(4, Nop)
+    (* :addloop *)
+    (* beqz r1 :done *)
   | 104 => Some(4, If (BinOp OP_EQ (Var R_R1) (Word 0 32)) (Jmp (Word 120 32)) (Nop))
+    (* sub r1 0x1 *)
   | 108 => Some(4, Move R_R1 (BinOp OP_MINUS (Var R_R1) (Word 1 32)))
+    (* add r2 0x1 *)
   | 112 => Some(4, Move R_R2 (BinOp OP_PLUS (Var R_R2) (Word 1 32)))
+    (* jmp :addloop *)
   | 116 => Some(4, Jmp (Word 104 32))
+    (* :loop *)
+    (* mov r2 r0 *)
   | 120 => Some(4, Move R_R0 (Var R_R2))
   | _ => None
   end.
@@ -159,7 +170,7 @@ Definition addloop_exit (t:trace) :=
 Theorem addloop_welltyped : welltyped_prog pil32typctx addloop.
 Proof. Picinae_typecheck. Qed.
 
-(* TODO: I (ilan) made this tactic, should add it to Picinae_ISA *)
+(* TODO: I (ilan) made this tactic, Kevin says there is a better way. *)
 Ltac bound_of MDL V :=
   let H := fresh "BOUND" in
   let opt_w := eval vm_compute in (archtyps V) in
@@ -284,11 +295,19 @@ End AddloopAndBeyond.
 Module Addloop'.
 Definition addloop (s:store) (a:addr) : option (N * stmt) :=
   match a with
+  (* li r3 0x1 *)
   | 100 => Some(4, Move (R_R3) (Word 1 32))
+  (* :loop *)
+  (* beqz r1 :exit *)
   | 104 => Some(4, If (BinOp OP_EQ (Var R_R1) (Word 0 32)) (Jmp (Word 120 32)) (Nop))
+  (* sub r1 r1 r3 *)
   | 108 => Some(4, Move R_R1 (BinOp OP_MINUS (Var R_R1) (Var R_R3)))
+  (* add r2 r2 r3 *)
   | 112 => Some(4, Move R_R2 (BinOp OP_PLUS  (Var R_R2) (Var R_R3)))
+  (* jmp :loop *)
   | 116 => Some(4, Jmp (Word 104 32))
+  (* :exit *)
+  (* mov r0 r2 *)
   | 120 => Some(4, Move R_R0 (Var R_R2))
   | _ => None
   end.
@@ -318,6 +337,408 @@ Proof.
 Admitted.
 End Addloop'.
 
-
 End Addloop.
+
+(** Exercise:4 stars, standard, optional (sumton)
+
+    Prove the following iterative sum adds up to the closed form expression
+   [(n*(n+1))/2 mod 2^32] when n>1 is given as input to R_R1. *)
+Module SumToN.
+Definition sumton (s:store) (a:addr) : option (N * stmt) :=
+  match a with
+  (* li r3 0x1 *)
+  | 100 => Some(4, Move (R_R3) (Word 1 32))
+  (* li r2 0x0 *)
+  | 104 => Some(4, Move (R_R2) (Word 0 32))
+  (* :loop *)
+  (* blt r1 r3 :exit *)
+  | 108 => Some(4, If (BinOp OP_LT (Var R_R1) (Var R_R3)) (Jmp (Word 124 32)) (Nop))
+  (* add r2 r2 r3 *)
+  | 112 => Some(4, Move R_R2 (BinOp OP_PLUS (Var R_R2) (Var R_R3)))
+  (* add r3 r3 0x1 *)
+  | 116 => Some(4, Move R_R3 (BinOp OP_PLUS (Var R_R3) (Word 1 32)))
+  (* jmp :loop *)
+  | 120 => Some(4, Jmp (Word 108 32))
+  (* :exit *)
+  (* mov r0 r2 *)
+  | 124 => Some(4, Move R_R0 (Var R_R2))
+  (* ret *)
+  | 128 => Some(4, Jmp (Var R_LR))
+  | _ => None
+  end.
+
+Theorem sumton_welltyped : welltyped_prog pil32typctx sumton.
+Proof. Picinae_typecheck. Qed.
+
+Section Invs.
+  (* CHANGE THESE *)
+  Variable s : store.
+  Definition Entry t xs' := startof t xs' = (Addr 100, s).
+  Definition Models := models pil32typctx s.
+  Definition Init t xs' n := Entry t xs' /\ Models /\ s R_R1 = n.
+
+  Definition postcondition s' n := s' R_R0 = ((n * (n+1)) / 2) mod 2^32.
+
+  Definition Invs n (t:trace) := match t with (Addr a, s)::_ =>
+    match a with
+    | 100 => Some (s R_R1 = n)
+    | 116 => Some (exists r2 r3, s R_R1 = n /\ s R_R2 = r2 /\ s R_R3 = r3
+                  /\ r3 <= n /\ r2 = ((r3*(1+r3))/2) mod 2^32)
+    | 128 => Some (postcondition s n)
+    | _ => None
+    end | _ => None end.
+
+  Definition exit (t:trace) := match t with (Addr 128,_)::_ => true | _=> false end.
+
+End Invs.
+
+Lemma mod_smaller:
+  forall n a b, b <> 0 -> n < a mod b -> n < b.
+Proof.
+  intros n a b NZ H.
+  transitivity (a mod b);[assumption| now apply N.mod_lt].
+Qed.
+
+Lemma even_div2_mul2 :
+  forall x, N.even x = true -> 2*(x/2) = x.
+Proof.
+Admitted.
+
+Lemma eq_mod_eq:
+  forall a b c, a = c -> a mod b = c mod b.
+Proof.
+  intros; now subst.
+Qed.
+
+Theorem sumton_partial_correctness:
+  forall (s:store) t xs' (n:N) (INIT : Init s t xs' n),
+  satisfies_all sumton (Invs n) exit (xs'::t).
+Proof.
+  (* FILL IN HERE *)
+  Local Ltac step := pil32_step.
+  intros s t xs' n (ENTRY & MDL & N).
+  apply prove_invs.
+
+  (* Base Case *)
+  simpl. rewrite ENTRY. step. assumption.
+
+  (* Inductive Case *)
+  intros.
+  eapply startof_prefix in ENTRY; try eassumption.
+  eapply preservation_exec_prog in MDL; try (eassumption || apply sumton_welltyped).
+  clear - PRE MDL. rename t1 into t; rename s1 into s.
+  destruct_inv 32 PRE.
+
+
+  (* 100 -> 128; 116 *)
+  step. step. step. step.
+    (* 128 *)
+    rewrite N.ltb_lt, N.lt_1_r in BC. rewrite BC; subst. now cbv.
+    (* 116 *)
+    step. rewrite N.ltb_ge in BC.
+    repeat (eexists || reflexivity || lia || split).
+
+  (* 116 -> 116; 128 *)
+  destruct PRE as (r2 & r3 & N & R2 & R3 & LE & IH).
+  step. step. step; step.
+    (* 128 *)
+    rewrite N.ltb_lt in BC. destruct (N.lt_ge_cases r3 (2^32-1)) as [Lt | Ge].
+      (* r3 < 2^32 - 1 *)
+      rewrite N.mod_small in BC by lia; assert (EQ:r3=n) by lia. rewrite EQ in *. rewrite IH.
+      clear N R2 R3 EQ MDL t0 t s IH r2 r3. now rewrite N.add_comm.
+      (* r3 >= 2^32 - 1 - contradiction on the exit condition because the loop would never terminate *)
+      (* TODO: this can be clearer... *)
+      exfalso.
+      assert (R3LT:=@models_var R_R3 archtyps s MDL). cbn in R3LT, Ge.
+      rewrite R3 in *.
+      Search N.modulo N.lt.
+      Search (_ < _ mod _)  -"msub".
+      assert (CONTRA:(1+r3) mod 2^32 < r3). {
+        destruct (N.lt_trichotomy r3 4294967295) as [Lt3 | [Eq3 | Gt3]].
+        (* rewrite Eq3 in *. now cbv. *)
+      }
+      lia.
+    (* 116 *)
+    rewrite N.ltb_ge in BC.
+    repeat (eexists || lia || split).
+    clear N R2 R3 MDL s t0 t.
+    rewrite IH; clear IH.
+    replace ((1 + (r3 * (1 + r3) / 2) mod 2 ^ 32 + r3) mod 2 ^ 32) with
+            ((2 + 2 * r3 + (r3 * (1+r3))) mod 2 ^ 32) by admit.
+    replace (((1 + r3) mod 2 ^ 32 * (1 + (1 + r3) mod 2 ^ 32) / 2) mod 2 ^ 32) with
+            ((1+r3) * (2 + r3) mod 2^32) by admit.
+    apply eq_mod_eq. lia.
+Admitted.
+End SumToN.
+
+(** Exercise:4 stars, standard, optional (factorial)
+
+    Prove the following loop computes the lower 32 bits of the factorial
+    of the value initially in R_R3.*)
+Module Factorial.
+Fixpoint natfactorial (n:nat) :=
+  match n with O => 1 | S n' => (N.of_nat n) * (natfactorial n') end.
+
+Definition factorial (s:store) (a:addr) : option (N * stmt) :=
+  match a with
+    (* li r1 0x1 *)
+  | 100 => Some(4, Move R_R1 (Word 1 32))
+    (* beqz r3 :exit *)
+  | 104 => Some(4, If (BinOp OP_EQ (Var R_R3) (Word 0 32)) (Jmp (Word 140 32)) Nop)
+    (* li r2 0x1 *)
+  | 108 => Some(4, Move R_R2 (Word 1 32))
+    (* nop *)
+  | 112 => Some(4, Nop)
+    (* :loop *)
+    (* beq r2 r3 :loop_done *)
+  | 116 => Some(4, If (BinOp OP_EQ (Var R_R2) (Var R_R3)) (Jmp (Word 136 32)) Nop)
+    (* mul r1 r1 r2 *)
+  | 120 => Some(4, Move R_R1 (BinOp OP_TIMES (Var R_R1) (Var R_R2)))
+    (* add r2 r2 0x1 *)
+  | 124 => Some(4, Move R_R2 (BinOp OP_PLUS (Var R_R2) (Word 1 32)))
+    (* jmp :loop *)
+  | 128 => Some(4, Jmp (Word 116 32))
+    (* nop *)
+  | 132 => Some(4, Nop)
+    (* :loop_done *)
+  | 136 => Some(4, Move R_R1 (BinOp OP_TIMES (Var R_R1) (Var R_R2)))
+    (* :exit *)
+    (* nop *)
+  | 140 => Some(4, Nop)
+  | _ => None
+  end.
+
+Theorem factorial_welltyped : welltyped_prog pil32typctx factorial.
+Proof. Picinae_typecheck. Qed.
+
+Section Invs.
+  (* CHANGE THESE *)
+  Variable s : store.
+  Definition Entry t xs' := startof t xs' = (Addr 100, s).
+  Definition Models := models pil32typctx s.
+  Definition Init t xs' r3 := Entry t xs' /\ Models /\ s R_R3 = r3.
+
+  Definition postcondition s' r3 := s' R_R1 = natfactorial (N.to_nat r3) mod 2^32.
+
+  Definition Invs r3 (t:trace) := match t with (Addr a, s)::_ =>
+    match a with
+    | 100 => Some (s R_R3 = r3)
+    | 124 => Some (s R_R1 = natfactorial (N.to_nat (s R_R2)) mod 2^32
+                  /\ s R_R2 < s R_R3 /\ s R_R3 = r3 /\ 0 < r3)
+    | 140 => Some (postcondition s r3)
+    | _ => None
+    end | _ => None end.
+
+
+  Definition exit (t:trace) := match t with (Addr 140, _)::_ => true | _ => false end.
+
+End Invs.
+
+Lemma natfactorial_pred:
+  forall n, natfactorial n * N.of_nat (S n) = natfactorial (S n).
+Proof.
+  induction n.
+  - reflexivity.
+  - unfold natfactorial at 2. rewrite N.mul_comm, N.mul_cancel_l; try lia.
+    rewrite <-IHn, N.mul_comm, N.mul_cancel_l; try lia.
+    reflexivity.
+Qed.
+
+
+Lemma S_to_nat :
+  forall n, N.to_nat (1+n) = S (N.to_nat n).
+Proof.
+  intros. now rewrite N.add_1_l, N2Nat.inj_succ.
+Qed.
+
+Lemma Nsucc_S :
+  forall n, N.succ n = N.of_nat (S (N.to_nat n)).
+Proof.
+  intros.
+  now rewrite Nat2N.inj_succ, N2Nat.id.
+Qed.
+
+Lemma mod_mono_r :
+  forall x b y, x < y -> x mod b < y.
+Proof.
+  intros. eapply N.le_lt_trans.
+  apply N.Div0.mod_le.
+  assumption.
+Qed.
+
+Theorem factorial_partial_correctness:
+  forall (s:store) t xs' (r3:N) (INIT : Init s t xs' r3),
+  satisfies_all factorial (Invs r3) exit (xs'::t).
+Proof.
+  Local Ltac step := pil32_step.
+  intros s t xs' r3 (ENTRY & MDL & R3).
+
+  apply prove_invs.
+
+  (* Base Case *)
+  simpl. rewrite ENTRY. step.  assumption.
+
+  (* Inductive Case *)
+  (* Explain the current proof obligation *)
+  intros.
+  eapply startof_prefix in ENTRY; try eassumption.
+  eapply preservation_exec_prog in MDL; try (eassumption || apply factorial_welltyped).
+  clear - PRE MDL. rename t1 into t; rename s1 into s.
+  destruct_inv 32 PRE.
+
+
+  (* 100 -> 140 *)
+  step; step. apply Neqb_ok in BC. subst. rewrite BC. simpl. rewrite N.mod_small; lia.
+
+  (* 100 -> 140 ; 120 *)
+  step. step. step. step.
+    (* 140 *)
+    apply Neqb_ok in BC0; subst; rewrite <-BC0; simpl. rewrite N.mod_small; lia.
+    (* 124 *)
+    step. apply N.eqb_neq in BC; apply N.eqb_neq in BC0.
+    Search (_ [?x:=_] ?y) (?y<>?x).
+    rewrite update_frame, update_updated; try easy. simpl.
+    rewrite N.mod_small; split; lia.
+
+  (* 116 -> 140; 124*)
+  destruct PRE as (R1 & LT & R3 & R3B).
+  step. step. step. step.
+    (* 140 *)
+     rewrite N.eqb_eq in BC.
+    assert (R3LT:=@models_var R_R3 archtyps s MDL). cbn in R3LT.
+    rewrite N.mod_small in BC; try lia.
+    rewrite! R3 in *. rewrite BC.
+    assert (R2: s R_R2 = N.pred r3) by lia.
+    rewrite R2. Search (N.succ (N.pred _)). rewrite <-(N.succ_pred_pos r3 R3B) at 2 3.
+    remember (N.pred r3) as x; clear - x.
+    rewrite Nsucc_S. remember (N.to_nat x) as n.
+    rewrite natfactorial_pred, Nat2N.id. reflexivity.
+    (* 124 *)
+    step. rewrite N.eqb_neq in BC.
+    assert (R3LT:=@models_var R_R3 archtyps s MDL). cbn in R3LT.
+    rewrite N.mod_small in BC; try lia.
+    remember (s R_R2) as r2; remember (s R_R1) as r1; rewrite R3 in *. clear Heqr1 Heqr2 R3 MDL t0 t.
+    repeat (split || lia).
+    rewrite update_frame, update_updated; try easy.
+    rewrite (N.mod_small (1+r2)) by lia.
+    rewrite! S_to_nat. unfold natfactorial at 2. fold natfactorial. rewrite N.mul_comm.
+    rewrite <-Nsucc_S, <- N.add_1_l. reflexivity.
+    (* destruct (N.lt_trichotomy (1+r2) r3) as [Lt | [Eq | Gt]]; try lia.
+       apply mod_mono_r. assumption.*)
+Qed.
+End Factorial.
+
+
+(** **** Exercise:4 stars, standard, recommended (wcscpy_partial_correctness)
+
+    Specify and prove the partial correctness of this simplified wcscpy
+    implementation.  This is the first usage of memory in this tutorial, and not
+    only that, but of memory-writes.  We've placed the invariants at the locations
+    we used to prove this correct, and left some of the loop-invariant intact with
+    additional explanation below.
+
+    You'll find many abstractions provided by Picinae are useful for this exercise.
+    Below is a complete list of what we used;  you can find more details about
+    these abstractions in the chapter [AbsAndPracs].
+
+      * [wstrlen] (wrapped up in the [strlen'] definition below)
+      * [wnilfree]
+      * [overlap] and [~ overlap]
+      * mem_region_unchanged
+*)
+Module wcscpy.
+(** r1 - pointer to source wide character string being copied.
+    r0 - pointer to destination *)
+Definition wcscpy (s:store) (a:addr) : option (N * stmt) :=
+  match a with
+  (* 0x00100000: mov r2,#0x0 *)
+  | 1048576 => Some (4, Move R_R2 (Word 0 32))
+
+  (* 0x00100004: ldr r3,[r1, r2, LSL #0x0] *)
+  | 1048580 => Some (4,
+    Move R_R3 (Cast CAST_UNSIGNED 32 (Load (Var V_MEM32)
+      (BinOp OP_PLUS (Var R_R1) (BinOp OP_LSHIFT (Var R_R2) (Word 0 32))) LittleE 4)))
+
+  (* 0x00100008: str r3,[r0, r2, LSL #0x0] *)
+  | 1048584 => Some (4,
+    Move V_MEM32 (Store (Var V_MEM32)
+    (BinOp OP_PLUS (Var R_R0) (BinOp OP_LSHIFT (Var R_R2) (Word 0 32)))
+    (Var R_R3)
+    LittleE 4)
+  )
+
+  (* 0x0010000c: add r2,r2,#0x4 *)
+  | 1048588 => Some (4,
+    Move R_R2 (BinOp OP_PLUS (Var R_R2) (Word 4 32)))
+
+  (* 0x00100010: cbnz r3,0x00100004 *)
+  | 1048592 => Some (4,
+    If (BinOp OP_NEQ (Var R_R3) (Word 0 32)) (
+      Jmp (Word 1048580 32)
+    ) (* else *) (
+      Nop
+    )
+  )
+
+  (* 0x00100014: ret *)
+  | 1048596 => Some (4, Nop)
+
+  | _ => None
+  end.
+
+Theorem wcscpy_welltyped : welltyped_prog pil32typctx wcscpy.
+Proof. Picinae_typecheck. Qed.
+
+Definition strlen' := wstrlen 32 LittleE.
+
+Section Invs.
+  Variable s:store.
+  Variable mem psrc pdest len:N.
+  (* CHANGE THESE *)
+  Definition Entry t xs' := startof t xs' = (Addr 0x00100000, s).
+  Definition Models := models pil32typctx s.
+  (** Replace the [True] in Init with your own initial conditions *)
+  Definition Init t xs' := Entry t xs' /\ Models /\
+    s V_MEM32 = mem /\ s R_R0 = pdest /\ s R_R1 = psrc
+    /\ True.
+
+  (** Replace the [True] in the postcondition with your own initial conditions *)
+  Definition postcondition (s:store) :=
+    exists m, s V_MEM32 = m /\ True.
+
+  Definition Invs (t:trace) := match t with (Addr a, s)::_ =>
+  match a with
+  | 0x00100000 => Some (s V_MEM32 = mem /\ s R_R0 = pdest /\ s R_R1 = psrc
+                        /\ True)
+  (** TODO: Explain the exists m, s V_MEM32 = m clause *)
+  | 0x00100004 => Some (exists m, s V_MEM32 = m
+                        /\ strlen' m psrc len
+                        /\ True)
+  | 0x00100014 => Some (postcondition s)
+  | _ => None end | _ => None end.
+
+  Definition exit (t:trace) := match t with (Addr 0x00100014,_)::_ => true | _ => false end.
+
+End Invs.
+
+Theorem wcscpy_partial_correctness:
+  forall (s:store) t xs' (mem psrc pdest len:N) (INIT : Init s mem psrc pdest t xs'),
+  satisfies_all wcscpy (Invs mem psrc pdest len) exit (xs'::t).
+Proof.
+  Local Ltac step := pil32_step.
+  intros s t xs' mem psrc pdest len (ENTRY & MDL & MEM & LEN & NOV).
+  apply prove_invs.
+
+  (* Base Case *)
+  simpl. rewrite ENTRY. step. repeat (assumption || split).
+
+  (* Inductive Case *)
+  (* Explain the current proof obligation *)
+  intros.
+  eapply startof_prefix in ENTRY; try eassumption.
+  eapply preservation_exec_prog in MDL; try (eassumption || apply wcscpy_welltyped).
+  clear - PRE MDL. rename t1 into t; rename s1 into s.
+  destruct_inv 32 PRE.
+Abort.
+End wcscpy.
 
