Picinae_auto.v
@@ -1,0 +1,61 @@
+(* Picinae: Platform In Coq for INstruction Analysis of Executables       ZZM7DZ
+                                                                          $MNDM7
+   Copyright (c) 2025 Kevin W. Hamlen            ,,A??=P                 OMMNMZ+
+   The University of Texas at Dallas         =:$ZZ$+ZZI                  7MMZMZ7
+   Computer Science Department             Z$$ZM++O++                    7MMZZN+
+                                          ZZ$7Z.ZM~?                     7MZDNO$
+                                        ?Z8ZO7.OM=+?                     $OMO+Z+
+   Any use, commercial or otherwise       ?D=++M++ZMMNDNDZZ$$Z?           MM,IZ=
+   requires the express permission of        MZZZZZZ+...=.8NOZ8NZ$7       MM+$7M
+   the author.                                 ?NNMMM+.IZDMMMMZMD8O77     O7+MZ+
+                                                     MMM8MMMMMMMMMMM77   +MMMMZZ
+                                                     MMMMMMMMMMMZMDMD77$.ZMZMM78
+                                                      MMMMMMMMMMMMMMMMMMMZOMMM+Z
+   Automation Extensions Module:                       MMMMMMMMMMMMMMMMM^NZMMN+Z
+   * rewriting store infoormation.                      MMMMMMMMMMMMMMM/.$MZM8O+
+   * lia pre-processing configuration                    MMMMMMMMMMMMMM7..$MNDM+
+                                                          MMDMMMMMMMMMZ7..$DM$77
+                                                           MMMMMMM+MMMZ7..7ZM~++
+                                                            MMMMMMMMMMM7..ZNOOMZ
+   To compile this module, first load and compile:           MMMMMMMMMM$.$MOMO=7
+   * Picinae_core                                             MDMMMMMMMO.7MDM7M+
+   * Picinae_theory                                            ZMMMMMMMM.$MM8$MN
+   * Picinae_statics                                           $ZMMMMMMZ..MMMOMZ
+   Then compile this module with menu option                    ?MMMMMM7..MNN7$M
+   Compile->Compile_buffer.                                      ?MMMMMZ..MZM$ZZ
+                                                                  ?$MMMZ7.ZZM7DZ
+                                                                    7MMM$.7MDOD7
+                                                                     7MMM.7M77ZZ
+                                                                      $MM78ZDZ7Z
+                                                                        MM8D$7Z7
+                                                                        MM7O$$+Z
+                                                                         M 7N8ZD
+ *)
+
+Require Import NArith.
+Require Import Picinae_theory.
+Require Import Picinae_statics.
+Require Export Lia ZifyN ZifyBool.
+Open Scope N.
+
+Module PicinaeAuto (IL: PICINAE_IL) (TIL: PICINAE_THEORY IL) (SIL: PICINAE_STATICS IL TIL).
+Import SIL.
+
+(** Eliminate the store by rewriting the expressions stored in registers and
+    inferring their bounds from the type context. *)
+Global Ltac elimstore :=
+  repeat lazymatch goal with
+  | [ H: ?s ?v = _, MDL: models ?typs ?s |- _] =>
+      let Hyp := fresh "SBound" in
+      pose proof (Hyp:=models_var v MDL); cbv -[N.lt N.pow] in Hyp;
+      (** Keep limit if bitwidth is small; if it is large lia will hang. *)
+      match type of Hyp with
+      | _ < 2 ^ ?w => assert (temp:(w <=? 256) = true) by reflexivity; clear temp
+      | _ => clear Hyp
+      end;
+      try rewrite H in *; clear H; try clear s MDL
+  end.
+
+Global Ltac Zify.zify_pre_hook ::= elimstore; unfold msub in *.
+
+End PicinaeAuto.
