tutorial/AbsAndPracs.v
@@ -1,0 +1,516 @@
+(** * Abstractions and Practices *)
+
+(* ################################################################# *)
+(** * Introduction *)
+
+(** This chapter surveys proof practices and Picinae-provided abstractions
+    that are very useful for completing proofs and specifying readable
+    properties.  This chapter can be skimmed once and used as a reference/extended
+    documentation.  If you ever find yourself thinking "there's got to be an
+    easy/easier way to do this!" or "surely someone else has solved this!" then
+    refer to this chapter.  It is likely there is an abstraction, a lemma, or
+    a standard practice for what you need.  And if there isn't, email
+    the author with your proposed solution.
+
+    Abstractions covered:
+
+      * memory: [getmem], [setmem], [xbits]
+      * memory safety: [overlap], [mem_region_unchanged],
+      * strings: [nilfree], [strlen], [wnilfree], [wstrlen]
+
+    Practices covered:
+
+      * lia with ZifyN
+      * psimpl
+      * proofs by contradiction with N.lt_trichotomy and friends
+      * equality over N by bitwise inspection 
+
+    (* TODO: add a Picinae themed Search tutorial section and link to this tutorial
+       there instead. *)
+    Additionally, you'll find it very useful to understand how to use the
+    Search command effectively.  The community has a great tutorial for this:
+    https://rocq-prover.github.io/platform-docs/features/tutorial_search_for_lemma.html
+    *)
+
+(* ################################################################# *)
+(** * Setting It Up *)
+
+Require Import NArith.
+Require Import Utf8.
+Open Scope N.
+
+(* ################################################################# *)
+(** * Practices *)
+
+(** We begin this chapter by covering common proving practices, which will
+    immediately help with some of the abstraction exercises.
+
+    First, and most importantly is [lia], Rocq's builtin linear integer
+    arithmetic solver.  Lia solves arithmetic goals such as equality and
+    comparison, and proves arbitrary goals by contradiction by finding
+    arithmetic inconsistencies in the hypothesis space.  Here we import [lia]
+    simply with [Require Import Lia.], but Picinae imports it through its
+    architecture files.  I.e., [Require Import Picinae_pilbox32.] will import
+    and configure [Lia] for you. *)
+
+Require Import Lia.
+
+(** Some basic examples of proving easy goals. *)
+Goal 32 > 2. lia. Qed.
+
+Goal forall x (LT: x < 2^30), x + 4 < 2^32. lia. Qed.
+
+Goal forall w x y z
+  (LTwx: w < x) (LTxy: x < y)
+  (LTyz: y < z) (LTzw: z < w), False.
+lia. Qed.
+
+(** The lia decision procedure is powerful but has some important limitations.
+    It performs propositional reasoning: it is able to destruct conjunctions,
+    disjunctions, and reason about implications, negations, and formulaic
+    rewrites.  However, it does not handle exponentiation by a variable,
+    e.g., 2 ^ w, and does not natively handle some common functions,
+    e.g., N.leb and N.mod.
+
+    We can make Lia even more powerful by importing ZifyBool and ZifyNat.  Zify,
+    read Z-e-fy, is Lia's preprocessing procedure which turns [N] and [nat]
+    values into [Z] integers.  As a Picinae user you won't need to touch it
+    directly unless you want to disable Picinae's custom preprocessing with
+    [Ltac Zify.zify_pre_hook ::= idtac.] *)
+
+Goal forall x (EQ: N.ltb x 3 = true), x < 3.
+intros.
+Fail lia. Abort.
+
+Require Import ZifyBool.
+
+Goal forall x (EQ: N.ltb x 3 = true), x < 3.
+lia. Qed.
+
+Goal forall x, x mod 2^32 < 2^32.
+Fail lia. Abort.
+
+Require Import ZifyN.
+
+Goal forall x, x mod 2^32 < 2^32.
+lia. Qed.
+
+(** Lia cannot handle arbitrary moduli, just like it cannot handle
+    arbitrary exponentiation. *)
+Goal forall x w, x mod w < w.
+Fail lia. Abort.
+
+(** But it can figure it out if there is enough information. *)
+Goal forall x w (LO: 3 < w) (HI: w < 13), x mod w < w.
+lia. Qed.
+
+Require Import Picinae_pilbox32.
+Import PIL32Notations.
+
+Goal forall len sublen (SUBLT : sublen < len),
+      4 * sublen + 4 <= 4 + 4 * len.
+lia. Qed.
+
+Goal forall len sublen i (SUBLT : sublen < len) (LT : i < sublen),
+      4 * i + 4 <= 4 + 4 * len.
+lia. Qed.
+
+Goal  forall r3 n
+        (LE : r3 <= n)
+        (BC : n < 1 + r3),
+      r3 = n.
+lia. Qed.
+
+
+Goal  forall n r3
+        (LE : r3 <= n)
+        (BC : n < 1 ⊕ r3)
+        (Ge : 2^32 - 1 <= r3),
+      False.
+lia. Qed.
+
+Goal  forall len sublen i
+        (SUBLT : sublen < len)
+        (LENLT : len < 2 ^ 30)
+        (LT : i < sublen),
+      4 + (4 * sublen ⊕ (2 ^ 32 - (4 * i ⊕ 4))) + 4 <= 2 ^ 32.
+intros.
+lia. Qed.
+
+Goal forall n r2 r3
+  (LE : r3 <= n)
+  (BC : 1 ⊕ r3 <= n)
+  (IH : r2 = (r3 * (1 + r3) / 2) mod 2 ^ 32 ∧ n < 2 ^ 32 - 1 ∨ n = 2 ^ 32 - 1),
+1 + r2 ⊕ r3 = ((1 ⊕ r3) * (1 + (1 ⊕ r3)) / 2) mod 2 ^ 32 ∧ n < 4294967295
+∨ n = 4294967295.
+intros.
+lia. Qed.
+
+(** Picinae can extend lia with a preprocessing step allowing it to understand
+    Picinae's definitions (e.g., msub) and store abstraction.  At present this
+    is a new feature and not incorporated in every architecture.  The file
+    Picinae_auto.v defines and configures this automation. To enable it,
+    instantiate the module defined therein in the Picinae arch specification
+    and export it.  See Picinae_pilbox32.v for an example. *)
+
+Goal forall s x (MDL: models pil32typctx s) (X: s R_R0 = x), x < 2^32.
+lia. Qed.
+
+(* ================================================================= *)
+
+(** ** Psimpl *)
+
+(** Psimpl, short for Picinae simplifier, simplifies expressions typically
+    appearing in Picinae proofs including types such as N, Bool, and store,
+    and functions such as (store) update and getmem/setmem. *)
+
+(* TODO: why are we getting a `frontend verification needing optimization` message
+   when using psimpl here? Coq 8.20.0 *)
+Goal forall s n, (s[R_R2 := (n * (1 + n) / 2) mod 2 ^ 32][R_R1 := n][R_R3 :=
+ 1 ⊕ n][R_R0 := (n * (1 + n) / 2) mod 2 ^ 32]) R_R0 =
+(n * (n + 1) / 2) mod 2 ^ 32.
+intros. psimpl. lia. Qed.
+
+Goal forall s n, (s[R_R2 := (n * (1 + n) / 2) mod 2 ^ 32][R_R1 := n][R_R3 :=
+ 1 ⊕ n][R_R0 := (n * (1 + n) / 2) mod 2 ^ 32]) R_R1 = n.
+intros. psimpl. reflexivity. Qed.
+
+
+(* ================================================================= *)
+
+(** ** Proofs by contradiction *)
+
+(** Many proofs are better solved by contradiction than by construction, and a
+    common way to start these is by case analysis on the comparison of two
+    constants.
+
+    [[
+   Search N "cases".
+
+    N.le_ge_cases: ∀ n m : N, n <= m ∨ m <= n
+
+    N.lt_ge_cases: ∀ n m : N, n < m ∨ m <= n
+
+    N.le_gt_cases: ∀ n m : N, n <= m ∨ m < n
+
+   ...
+
+   Check N.lt_trichotomy.
+
+    N.lt_trichotomy
+        : ∀ n m : N, n < m ∨ n = m ∨ m < n
+
+   Check N.eq_dec.
+
+    N.eq_dec
+        : ∀ n m : N, {n = m} + {n ≠ m}
+   ]]
+
+    The lemma, e.g., N.lt_ge_cases, is chosen and specialized so that in
+    one case the goal is trivial (it is assumed), and in the other case the
+    assumption allows the prover to construct a contradiction, i.e., prove [False].
+*)
+
+(** **** Exercise:1 star, standard, optional (nflen_lt)
+
+  [nflen_lt] states that a nilfree region in some 64-bit memory [m] with
+  a zero byte has a length less than 2^64.  Prove it by contradiction using
+  psimpl and lia.  Can you prove this holds for any w-bit memory?
+
+  [nilfree] is Picinae's abstraction for memory regions without zero-bytes,
+  it is discussed in more depth below. *)
+Lemma nflen_lt:
+  forall m p len z
+  (NF: nilfree 64 LittleE m p len)
+  (Z:  getmem 64 LittleE 1 m z = 0),
+  len < 2 ^ 64.
+Proof.
+Abort.
+
+(* ================================================================= *)
+
+(** ** Equality proofs by bitwise inspection *)
+
+(** Think about it, if two binary numbers have the same digit in every position,
+    then they must have the same value.  So you can prove that two integer-valued
+    expressions are equal, such as [x mod 2^3] and [N.land x 7], are equal by
+    proving that the bits in each position are equal.  The typical proof appeals
+    to this fact, [N.bits_inj] or [N.bits_inj_0], and reasons about the value of each
+    bit by repeated applications of "spec" bit-specifcation theorems.
+
+    * *)
+
+Example x_mod_8__x_land_7:
+  forall x, x mod 2^3 = N.land x 7.
+Proof.
+  intros.
+  apply N.bits_inj.
+  (* The goal now asks us to prove the two expressions are functionally equivalent. *)
+  unfold N.eqf. intro i.
+
+  (* We reason that the 3rd index ([i]=3) and greater are 0 and indices 0-2 are
+     equal to what they are in [x].  Thus we proceed by case analysis on which
+     index, splitting into the cases \[0,2\] and \[3,inf). *)
+  destruct (N.lt_ge_cases i 3) as [LO | HI].
+{
+  (* Appeal to the digit being the same as x because the index is less than
+     the power of the power-of-2 modulus. *)
+  rewrite N.mod_pow2_bits_low; try assumption.
+  (* Appeal to the bit-spec of logical and--N.testbit of a digit returns true iff
+     it returns true for both sides of the N.land expression. *)
+  rewrite N.land_spec.
+  (* Replace 7 with 0b111, expressed as [N.ones 3], to capture the significance
+     of the number--specifcally, that it is a sequence of 1-bits... *)
+  replace 7 with (N.ones 3); try reflexivity.
+  (* ... and use this to show the rhs of the logical-and always evaluates
+     to true... *)
+  rewrite N.ones_spec_low; try assumption.
+  (* ... so the expression is equal only to the lhs. *)
+  rewrite Bool.andb_true_r.
+  reflexivity.
+}
+{
+  (* Appeal to the digit being zero because the index is greater than
+     the power of the power-of-2 modulus. *)
+  rewrite N.mod_pow2_bits_high; try assumption.
+  (* Break apart the logical-and on the rhs of the goal. *)
+  rewrite N.land_spec.
+  (* Again replace 7 with its [N.ones] representation. *)
+  replace 7 with (N.ones 3); try reflexivity.
+  (* This time appeal to the index being higher than the number of ones in
+     [N.ones], so the testbit evaluates to false. *)
+  rewrite N.ones_spec_high; try assumption.
+  (* And the boolean-and evaluates to false. *)
+  rewrite Bool.andb_false_r.
+  reflexivity.
+}
+Qed.
+
+(** **** Exercise:1 star, standard, optional (land_ones_proof)
+
+    Prove the generalization of the above theorem.  Try not to look at its proof,
+    instead use [Search] to find the needed helper lemmas.  You may not use the
+    N.land_ones theorem from the standard library. *)
+
+Theorem land_ones:
+  forall x w, x mod 2^w = N.land x (N.ones w).
+Proof.
+Abort.
+
+(** **** Exercise:1 star, standard, optional (Nshiftr_land_ones_high)
+
+   Prove the following using [N.bits_inj_0], the specialization of [N.bits_inj]
+   when the right-hand-side is zero. *)
+Lemma Nshiftr_land_ones_high:
+  forall a n m, m <= n -> (a << n) .& (N.ones m) = 0.
+Proof.
+Abort.
+
+(** **** Exercise:1 star, standard, optional (Nshiftr_land_high_nop)
+
+    Prove the following using N.bits_inj. *)
+Lemma Nshiftr_land_high_nop:
+  forall a b n m, n > m -> (a .| b << n) .& (N.ones m) = a .& (N.ones m).
+Proof.
+Abort.
+
+(** **** Exercise:1 star, standard, optional (xbits_lshift_0)
+
+    Prove the following. *)
+Lemma xbits_lshift_0:
+  forall n shift i j, i <= j -> j <= shift -> xbits (n << shift) i j = 0.
+Proof.
+Abort.
+
+(* ################################################################# *)
+(** * Abstractions *)
+
+(** ** Memory *)
+(** So far we've only considered arithmetic examples dealing exclusively with
+    the contents of registers.  When we start reasoning about data structures,
+    non-numeric data, and memory we need to introduce abstractions.  At the
+    most fundamental level we have Picinae's builtin abstraction for memory-access:
+    [getmem] and [setmem].  These abstract the notion of memory as an 8*2^w-bit
+    bitstring and allow us to handle byte-aligned big- and little-endian reads
+    and writes.
+
+    [[
+        Definition getmem w (e:endianness) len mem p : N := _.
+
+        Definition setmem w (e:endianness) len mem p v : memory := _.
+    ]]
+
+   Picinae treats memory as a bit-string that wraps around on itself.  A 2kb
+   read starting at the last kilobyte of 32-bit memory,
+   [getmem 32 _ 2048 mem (2^32-1024)], returns a value comprised of the first
+   and last kilobytes of [mem].  A write at an address beyond the w-bit addressable
+   memory is mapped to an in-bound address by taking the appropriate remainder modulo bytewidth
+   Writing four bytes starting twenty bytes beyond the memory address is the
+   equivalent to writing the same four bytes at address 20.  That is,
+   [setmem 32 _ 4 (2^32+20) v] is equivalent to [setmem 32 _ 4 20 v].
+
+   Memory writes return the updated memory.  This non-destructive approach
+   allows reasoning about memory in several different states, which is
+   absolutely necessary when programs interleave reads and writes.
+*)
+
+(** **** Exercise:1 star, standard, optional (setmem_4_w20_20)
+
+    Prove the assertion we made above about writing to memory beyond the
+    address space.  We start you off with a useful search.  Oh, and feel free
+    to import Lia at any time.
+ *)
+Theorem setmem_4_w20_20:
+  forall e mem v, setmem 32 e 4 mem (2^32+20) v = setmem 32 e 4 mem 20 v.
+Proof.
+  Search setmem -nilfree -"frame" -overlap.
+Abort.
+
+(** [getmem] and [setmem] are opaque at the typical user level, meaning you
+    cannot unfold or see their definitions.  Working with them requires you to
+    use the many getmem and setmem functions available in Picinae_theory.
+
+    [[
+      Search getmem in Picinae_theory.
+    ]]
+
+    If you need a property of [getmem] or [setmem] that does not exist, you can
+    prove it inside of Picinae_theory where you can unfold the definition.  This
+    should not be necessary.  For instance, proving a property by recursing over
+    the length of the read/write does not require unfolding the definition and
+    is facilitated by the [getmem_succ] and [setmem_succ] theorems.  To read
+    more about proofs by induction refer to the MemTheory section in
+    Picinae_theory.v. *)
+
+(** ** Strings *)
+
+(** Ascii nil-terminated strings are a simple datastructure.  Each byte is
+    treated as an ASCII character and the end of the string is marked by
+    the null character 0x00 (we use nil and null interchangably).  Technically,
+    we can reason about string functions and programs that operate on strings
+    without ever considering their semantics.  They are all encoded as bits
+    after all.  However developing a library of abstractions is very helpful
+    for reading the specifications and writing the proofs.
+
+    The [nilfree] proposition encodes what it means for a string starting at
+    [p] to have at least [len] non-nil characters.  Specifically, it states
+    that all indices [i] less than [len] into the string starting at [p] are
+    non-nil.  Remember that indices start at 0, so there are [len] unique
+    indices between 0 and [len-1] inclusive, and thus [len] characters.
+
+    FYI: most unix system will have a man page you can reference for the
+    Ascii characters and their encodings as numeric values.  Try running
+    [man ascii] in your terminal.
+ *)
+Module string_defs.
+
+Definition nilfree mem p len :=
+  forall w e i, i < len -> getmem w e 1 mem p <> 0.
+
+(** **** Exercise:1 star, standard, required (strlen_def)
+
+   Fill in a definition for the length of a nil-terminated string in memory
+   [mem] starting at location [p] using the definition for nilfree. *)
+
+Definition strlen (mem p len:N) : Prop := (* _FILL_IN_HERE_ *) True.
+
+(** **** Exercise:1 star, standard, optional (nilfree_lr_len)
+
+    Prove this lemma saying that there are no null characters before any index
+    inside of a string. *)
+Lemma nilfree_le_len :
+  forall mem p len k
+    (LEN : strlen mem p len)
+    (LE  : k <= len),
+    nilfree mem p k.
+Proof.
+Abort.
+
+(** **** Exercise:1 star, standard, optional (strlen_incr)
+
+    Prove this strlen lemma used in reasoning about the length of a string as
+    we discover new information about its characters.  It states that if we know
+    a character, possibly the nil-terminator, is not the nil-terminator then the
+    length of the string is greater than the index of this character. *)
+Lemma strlen_incr :
+  forall mem p len k
+    (LEN : strlen mem p len)
+    (LE : k <= len)
+    (NNULL : mem Ⓑ[ p + k ] <> 0),
+     k < len.
+Proof.
+Abort.
+
+(** **** Exercise:2 stars, standard, optional (wnilfree_sublen_eq_len)
+
+    Prove this lemma used in the wcscpy proof below without peeking at
+    Picinae_theory.  It states that the length, [sublen], of a nil-free substring
+    is the length of the entire string if there is a nil terminator at its
+    corresponding index. *)
+Lemma wnilfree_sublen_eq_len:
+  forall w e mem p len sublen
+    (NF: wnilfree w e mem p sublen)
+    (LEN: wstrlen w e mem p len)
+    (BC: getmem w e 4 mem (p+4*sublen) = 0),
+  sublen = len.
+Proof.
+Abort.
+
+End string_defs.
+
+(** ** Memory Safety *)
+
+(** Once we start reasoning about programs that modify code, e.g., the [wcscpy]
+    exercise in BasicLoops, it becomes necessary to reason about the memory safety
+    of programs.  In other words, we need a way to say that values read from two
+    different memories are the same, that the expected value was not overwritten
+    during an execution, or that it was correctly copied by a write or sequence
+    of writes.
+
+    The [overlap] and [mem_region_unchanged] abstractions are used for this purpose.
+    [Overlap] defines what it means for two memory regions specified by their initial
+    addresses and their lengths to overlap in a w-bit system, useful e.g., to define
+    that a destination buffer does not overlap with the source buffer.
+    [Mem_region_unchanged] is a shorthand for stating that the bytes in a specification
+    region of two different memories are the same, useful e.g., when we want to
+    describe a data structure as static.
+
+    In particular, the [getmem_noverlap] and [getmem_index_unchanged] theorems help
+    by rewriting memory accesses from modified memories to memory accesses from
+    unmodified memory, providing some non-overlapping conditions hold.  Often times
+    [getmem_noverla] is followed by a [noverlap_sum; lia] invocation to prove the
+    [~ overlap] condition.  When lia is not strong enough for this the intensive overlap
+    theory library is well equipped for reasoning about overlaps and non-overlaps at
+    a high level.
+
+    [[
+      Search overlap.
+    ]] *)
+
+(** **** Exercise:1 star, standard, optional (getmem_setmem_eq)
+
+   Prove the following lemma featuring [overlap]. *)
+
+Lemma getmem_setmem_eq:
+  forall mem e (a wraddr wrlen v min max : N)
+    (HEAD : min <= a <= max)
+    (NOV : ~ overlap 32 wraddr wrlen min (max + 8 - min)),
+  mem Ⓓ[ 4 + a ] = setmem 32 e wrlen mem wraddr v Ⓓ[ 4 + a ].
+Proof.
+  (* FILL IN HERE *)
+Abort.
+
+(** **** Exercise:1 star, standard, optional (wstrlen_same)
+
+   Prove the following lemma featuring [overlap]. *)
+
+Lemma wstreln_same:
+  forall psrc pdest len mem sublen
+    (LEN : wstrlen 32 LittleE mem psrc len)
+    (NOV : ¬ overlap 32 psrc (4 + 4 * len) pdest (4 + 4 * len))
+    (SUBLT : sublen < len),
+  wstrlen 32 LittleE
+    (mem [Ⓓ pdest + 4 * sublen := mem Ⓓ[ psrc + 4 * sublen ] ]) psrc len.
+Proof.
+  (* FILL IN HERE *)
+Abort.
